proof/crefine/ARM/Interrupt_C.thy
@@ -285,39 +285,97 @@ lemma mask_of_mask[simp]:
   apply (auto simp:word_size)
   done
 
-lemma invokeIRQControl_ccorres:
-  "ccorres (K (K \<bottom>) \<currency> dc) (liftxf errstate id (K ()) ret__unsigned_long_')
-      (invs' and cte_at' parent and (\<lambda>_. (ucast irq) \<le> (scast Kernel_C.maxIRQ :: word32)))
+lemma ucast_maxIRQ_le_eq:
+  "UCAST(10 \<rightarrow> 32) irq \<le> SCAST(32 signed \<rightarrow> 32) Kernel_C.maxIRQ \<Longrightarrow>
+   UCAST(10 \<rightarrow> 16) irq \<le> SCAST(32 signed \<rightarrow> 16) Kernel_C.maxIRQ"
+  apply (subst ucast_le_ucast[where 'a=16 and 'b=32, symmetric])
+  apply simp
+  by (clarsimp simp: ucast_up_ucast is_up Kernel_C.maxIRQ_def)
+
+lemma ucast_maxIRQ_le_eq':
+  "UCAST(10 \<rightarrow> 32) irq \<le> SCAST(32 signed \<rightarrow> 32) Kernel_C.maxIRQ \<Longrightarrow> irq \<le> maxIRQ"
+  apply (clarsimp simp: Kernel_C.maxIRQ_def maxIRQ_def)
+  by word_bitwise
+
+lemma invokeIRQControl_expanded_ccorres:
+  "ccorres (\<lambda>_ r. r = scast EXCEPTION_NONE) (ret__unsigned_long_')
+      (invs' and cte_at' parent and (\<lambda>_. (ucast irq) \<le> (scast Kernel_C.maxIRQ :: machine_word)))
       (UNIV \<inter> {s. irq_' s = ucast irq}
-                  \<inter> {s. controlSlot_' s = cte_Ptr parent}
-                  \<inter> {s. handlerSlot_' s = cte_Ptr slot}) []
-      (performIRQControl (IssueIRQHandler irq slot parent))
+            \<inter> {s. controlSlot_' s = cte_Ptr parent}
+            \<inter> {s. handlerSlot_' s = cte_Ptr slot}) hs
+      (do x <- setIRQState irqstate.IRQSignal irq;
+          cteInsert (capability.IRQHandlerCap irq) parent slot
+       od)
       (Call invokeIRQControl_'proc)"
-  apply (rule ccorres_gen_asm)
-  apply (cinit lift: irq_' controlSlot_' handlerSlot_')
-   apply (simp add: liftE_def bind_assoc return_returnOk)
+  apply (cinit' lift: irq_' controlSlot_' handlerSlot_')
    apply (ctac add: setIRQState_ccorres)
      apply csymbr
-     apply (ctac(no_vcg) add: cteInsert_ccorres)
-      apply (rule ccorres_return_CE, simp+)[1]
+     apply (rule ccorres_add_return2)
+     apply (ctac (no_vcg) add: cteInsert_ccorres)
+      apply (rule_tac P=\<top> and P'=UNIV in ccorres_from_vcg_throws)
+      apply (rule allI, rule conseqPre, vcg)
+      apply (clarsimp simp: return_def)
      apply wp+
-   apply (simp add: Collect_const_mem)
+   apply clarsimp
    apply (vcg exspec=setIRQState_modifies)
+  apply (clarsimp simp: is_simple_cap'_def isCap_simps valid_cap_simps' capAligned_def
+                        word_bits_def)
   apply (rule conjI)
-   apply (clarsimp simp: is_simple_cap'_def isCap_simps valid_cap_simps' capAligned_def)
-   apply (subst ucast_le_ucast[where 'a = 16 and 'b = 32,symmetric],simp)
-   apply (subst ucast_le_ucast_10_32[symmetric])
-   apply (auto simp:ucast_up_ucast is_up ARM.maxIRQ_def Kernel_C.maxIRQ_def word_bits_def )[1]
+   apply (fastforce simp: word_bits_def intro!: ucast_maxIRQ_le_eq ucast_maxIRQ_le_eq')
+  apply (simp add: invs_mdb' invs_valid_objs' invs_pspace_aligned')
+  apply (rule conjI)
+   apply (clarsimp simp: maxIRQ_def Kernel_C.maxIRQ_def)
+   apply unat_arith
   apply (clarsimp simp: Collect_const_mem ccap_relation_def cap_irq_handler_cap_lift
                         cap_to_H_def c_valid_cap_def cl_valid_cap_def
-                        word_bw_assocs mask_twice Kernel_C.maxIRQ_def ucast_ucast_a
+                        word_bw_assocs mask_twice maxIRQ_def Kernel_C.maxIRQ_def ucast_ucast_a
                         is_up ucast_ucast_b is_down)
   apply (subst less_mask_eq)
-    apply (rule le_m1_iff_lt[THEN iffD1,THEN iffD1])
-     apply simp
-    apply (erule order.trans,simp)
+   apply (rule le_m1_iff_lt[THEN iffD1,THEN iffD1])
+    apply simp
+   apply (erule order.trans, simp)
   apply (rule word_eqI)
   apply (simp add: nth_ucast word_size)
+  done
+
+lemma invokeIRQControl_ccorres:
+  "ccorres (K (K \<bottom>) \<currency> dc) (liftxf errstate id (K ()) ret__unsigned_long_')
+      (invs' and cte_at' parent and (\<lambda>_. (ucast irq) \<le> (scast Kernel_C.maxIRQ :: machine_word)))
+      (UNIV \<inter> {s. irq_' s = ucast irq}
+                  \<inter> {s. controlSlot_' s = cte_Ptr parent}
+                  \<inter> {s. handlerSlot_' s = cte_Ptr slot}) hs
+      (performIRQControl (Invocations_H.IssueIRQHandler irq slot parent))
+      (Call invokeIRQControl_'proc)"
+  unfolding performIRQControl_def
+  apply simp
+  apply (rule ccorres_liftE)
+  apply (rule ccorres_rel_imp)
+   apply (rule ccorres_guard_imp)
+     apply (rule invokeIRQControl_expanded_ccorres)
+    apply assumption
+   apply simp+
+  done
+
+lemma Arch_invokeIRQControl_ccorres:
+  "ccorres ((K (K \<bottom>)) \<currency> dc) (liftxf errstate id (K ()) ret__unsigned_long_')
+      (invs' and cte_at' parent and (\<lambda>_. (ucast irq) \<le> (scast Kernel_C.maxIRQ :: machine_word)))
+      (UNIV \<inter> {s. irq_' s = ucast irq}
+            \<inter> {s. handlerSlot_' s = cte_Ptr slot}
+            \<inter> {s. controlSlot_' s = cte_Ptr parent}
+            \<inter> {s. trigger_' s = from_bool trigger}) hs
+      (performIRQControl (ArchIRQControl (IssueIRQHandler irq slot parent trigger)))
+      (Call Arch_invokeIRQControl_'proc)"
+  unfolding ARM_H.performIRQControl_def IRQ_def
+  apply (cinit lift: irq_' handlerSlot_' controlSlot_' trigger_'
+               simp: ARM_H.performIRQControl_def IRQ_def)
+   apply (rule ccorres_liftE)
+   apply (ctac (no_vcg) add: setIRQTrigger_ccorres)
+     apply (rule ccorres_add_return2)
+     apply (ctac (no_vcg) add: invokeIRQControl_expanded_ccorres)
+       apply (rule_tac P=\<top> and P'=UNIV in ccorres_from_vcg_throws)
+       apply (rule allI, rule conseqPre, vcg)
+       apply (clarsimp simp: return_def)
+      apply (wpsimp simp: guard_is_UNIV_def)+
   done
 
 lemma unat_ucast_16_32:
@@ -354,20 +412,6 @@ lemma Platform_maxIRQ:
   "ARM.maxIRQ = scast Kernel_C.maxIRQ"
   by (simp add: ARM.maxIRQ_def Kernel_C.maxIRQ_def)
 
-lemma Arch_decodeIRQControlInvocation_ccorres:
-  "ccorres (intr_and_se_rel \<currency> dc) (liftxf errstate id (K ()) ret__unsigned_long_')
-      \<top> UNIV []
-     (Arch.decodeIRQControlInvocation label args srcSlot extraCaps
-        >>= invocationCatch thread isBlocking isCall (InvokeIRQControl o ArchIRQControl))
-     (Call Arch_decodeIRQControlInvocation_'proc)"
-  apply (cinit' simp: ARM_H.decodeIRQControlInvocation_def)
-   apply (simp add: throwError_bind invocationCatch_def
-              cong: StateSpace.state.fold_congs globals.fold_congs)
-   apply (rule syscall_error_throwError_ccorres_n)
-   apply (simp add: syscall_error_to_H_cases)
-  apply simp
-  done
-
 lemma liftME_invocationCatch:
   "liftME f m >>= invocationCatch thread isBlocking isCall f'
      = m >>= invocationCatch thread isBlocking isCall (f' \<circ> f)"
@@ -385,6 +429,10 @@ lemma maxIRQ_ucast_scast [simp]:
 lemma decodeIRQ_arch_helper: "x \<noteq> invocation_label.IRQIssueIRQHandler \<Longrightarrow>
          (case x of invocation_label.IRQIssueIRQHandler \<Rightarrow> f | _ \<Rightarrow> g) = g"
   by (clarsimp split: invocation_label.splits)
+
+lemma decodeIRQ_arch_helper': "x \<noteq> ArchInvocationLabel ARMIRQIssueIRQHandler \<Longrightarrow>
+         (case x of ArchInvocationLabel ARMIRQIssueIRQHandler \<Rightarrow> f | _ \<Rightarrow> g) = g"
+  by (clarsimp split: invocation_label.splits arch_invocation_label.splits)
 
 lemma Arch_checkIRQ_ccorres:
   "ccorres (syscall_error_rel \<currency> (\<lambda>r r'. irq \<le> scast Kernel_C.maxIRQ))
@@ -435,8 +483,180 @@ lemma unat_ucast_mask:
   apply simp
   done
 
+lemma Arch_decodeIRQControlInvocation_ccorres:
+  notes if_cong[cong]
+  shows
+  "interpret_excaps extraCaps' = excaps_map extraCaps \<Longrightarrow>
+   ccorres (intr_and_se_rel \<currency> dc) (liftxf errstate id (K ()) ret__unsigned_long_')
+       (invs' and (\<lambda>s. ksCurThread s = thread)
+              and sch_act_simple and ct_active'
+              and (excaps_in_mem extraCaps o ctes_of)
+              and cte_wp_at' (\<lambda>cte. cteCap cte = IRQControlCap) slot
+              and (\<lambda>s. \<forall>v \<in> set extraCaps. s \<turnstile>' fst v)
+              and sysargs_rel args buffer)
+       (UNIV
+            \<inter> {s. invLabel_' s = label} \<inter> {s. srcSlot_' s = cte_Ptr slot}
+            \<inter> {s. unat (length___unsigned_long_' s) = length args}
+            \<inter> {s. excaps_' s = extraCaps'}
+            \<inter> {s. buffer_' s = option_to_ptr buffer}) []
+     (Arch.decodeIRQControlInvocation label args slot (map fst extraCaps)
+        >>= invocationCatch thread isBlocking isCall (InvokeIRQControl o ArchIRQControl))
+     (Call Arch_decodeIRQControlInvocation_'proc)"
+  apply (cinit' lift: invLabel_' srcSlot_' length___unsigned_long_' excaps_' buffer_')
+   apply (simp add: ARM_H.decodeIRQControlInvocation_def invocation_eq_use_types
+               del: Collect_const
+               cong: StateSpace.state.fold_congs globals.fold_congs)
+   apply (rule ccorres_Cond_rhs)
+    apply (simp add: list_case_If2
+                del: Collect_const cong: call_ignore_cong)
+    apply (rule ccorres_rhs_assoc)+
+    apply csymbr+
+    apply (rule ccorres_Cond_rhs_Seq)
+     apply (simp add: word_less_nat_alt throwError_bind invocationCatch_def)
+     apply (rule ccorres_cond_true_seq)
+     apply (rule syscall_error_throwError_ccorres_n)
+     apply (simp add: syscall_error_to_H_cases)
+    apply csymbr
+    apply (rule ccorres_Cond_rhs_Seq)
+     apply (simp add: interpret_excaps_test_null excaps_map_def throwError_bind
+                      invocationCatch_def)
+     apply (rule syscall_error_throwError_ccorres_n)
+     apply (simp add: syscall_error_to_H_cases)
+    apply (simp add: interpret_excaps_test_null excaps_map_def
+                     word_less_nat_alt Let_def
+                del: Collect_const cong: call_ignore_cong)
+    apply (rule ccorres_add_return)
+    apply (ctac add: getSyscallArg_ccorres_foo[where args=args and n=0 and buffer=buffer])
+      apply csymbr
+      apply (rule ccorres_add_return)
+      apply (ctac add: getSyscallArg_ccorres_foo[where args=args and n=1 and buffer=buffer])
+        apply (rule ccorres_add_return)
+        apply csymbr
+        apply (ctac add: getSyscallArg_ccorres_foo[where args=args and n=2 and buffer=buffer])
+          apply (rule ccorres_add_return)
+          apply (ctac add: getSyscallArg_ccorres_foo[where args=args and n=3 and buffer=buffer])
+            apply (rule getSlotCap_ccorres_fudge_n[where vals=extraCaps and n=0])
+            apply (rule ccorres_move_c_guard_cte)
+            apply ctac
+              apply (rule ccorres_assert2)
+              apply (simp add: rangeCheck_def unlessE_def ARM.minIRQ_def
+                               ucast_nat_def word_le_nat_alt[symmetric]
+                               linorder_not_le[symmetric] Platform_maxIRQ
+                               length_ineq_not_Nil hd_conv_nth cast_simps
+                               maxIRQ_ucast_scast
+                          del: Collect_const cong: call_ignore_cong)
+              apply (simp add: split_def invocationCatch_use_injection_handler
+                               injection_handler_bindE bindE_assoc
+                          del: Collect_const)
+              apply (ctac add: ccorres_injection_handler_csum1[OF Arch_checkIRQ_ccorres])
+                 apply (simp add: injection_liftE)
+                 apply (simp add: liftE_bindE bind_assoc del: Collect_const)
+                 apply (ctac add: isIRQActive_ccorres)
+                   apply (simp add: from_bool_0 del: Collect_const)
+                   apply (rule ccorres_Cond_rhs_Seq)
+                    apply (simp add: throwError_bind invocationCatch_def whenE_def
+                                     injection_handler_throwError)
+                    apply (rule syscall_error_throwError_ccorres_n)
+                    apply (simp add: syscall_error_to_H_cases)
+                   apply (simp add: split_def invocationCatch_use_injection_handler
+                                    injection_handler_bindE bindE_assoc whenE_def
+                                    injection_handler_returnOk
+                               del: Collect_const)
+                   apply (ctac add: ccorres_injection_handler_csum1
+                                    [OF lookupTargetSlot_ccorres, unfolded lookupTargetSlot_def])
+                      apply (simp add: Collect_False split_def del: Collect_const)
+                      apply csymbr
+                      apply (ctac add: ccorres_injection_handler_csum1
+                                       [OF ensureEmptySlot_ccorres])
+                      apply (simp add: injection_handler_returnOk ccorres_invocationCatch_Inr
+                                       performInvocation_def bindE_assoc) using [[goals_limit=2]]
+                      apply (ctac add: setThreadState_ccorres)
+                      apply (ctac(no_vcg) add: Arch_invokeIRQControl_ccorres)
+                      apply (rule ccorres_alternative2)
+                      apply (rule ccorres_return_CE, simp+)[1]
+                      apply (rule ccorres_return_C_errorE, simp+)[1]
+                      apply (wp sts_invs_minor')+
+                      apply (simp add: Collect_const_mem)
+                      apply (vcg exspec=setThreadState_modifies)
+                      apply simp
+                      apply (rule ccorres_split_throws)
+                      apply (rule ccorres_return_C_errorE, simp+)[1]
+                      apply vcg
+                      apply simp
+                      apply (wp injection_wp_E [OF refl])
+                      apply (simp add: Collect_const_mem all_ex_eq_helper)
+                      apply (vcg exspec=ensureEmptySlot_modifies)
+                     apply simp
+                     apply (rule ccorres_split_throws)
+                      apply (rule ccorres_return_C_errorE, simp+)[1]
+                     apply vcg
+                    apply simp
+                    apply (wp injection_wp_E[OF refl] hoare_drop_imps)
+                   apply (simp add: Collect_const_mem all_ex_eq_helper)
+                   apply (vcg exspec=lookupTargetSlot_modifies)
+                  apply simp
+                  apply (wp hoare_drop_imps isIRQActive_inv)
+                 apply (simp add: Collect_const_mem all_ex_eq_helper)
+                 apply (vcg exspec=isIRQActive_modifies)
+                apply simp
+                apply (rule ccorres_split_throws)
+                 apply (rule ccorres_return_C_errorE, simp+)[1]
+                apply vcg
+               apply simp
+               apply (wp injection_wp_E[OF refl] checkIRQ_ret_good)
+              apply (simp add: Collect_const_mem all_ex_eq_helper)
+              apply (vcg exspec=Arch_checkIRQ_modifies)
+             apply (wp hoare_vcg_const_imp_lift |wp_once hoare_drop_imps)+
+            apply (simp add: Collect_const_mem all_ex_eq_helper)
+            apply vcg
+           apply wp
+          apply (simp add: Collect_const_mem all_ex_eq_helper)
+          apply (vcg exspec=getSyscallArg_modifies)
+         apply simp
+         apply wp
+        apply (simp add: Collect_const_mem all_ex_eq_helper)
+        apply (vcg exspec=getSyscallArg_modifies)
+       apply simp
+       apply wp
+      apply (simp add: Collect_const_mem all_ex_eq_helper)
+      apply (vcg exspec=getSyscallArg_modifies)
+     apply simp
+     apply wp
+    apply (simp add: Collect_const_mem all_ex_eq_helper)
+    apply (vcg exspec=getSyscallArg_modifies)
+   apply (clarsimp simp: decodeIRQ_arch_helper')
+   apply (simp add: throwError_bind invocationCatch_def)
+   apply (rule syscall_error_throwError_ccorres_n)
+   apply (simp add: syscall_error_to_H_cases)
+  apply (clarsimp simp: interpret_excaps_test_null excaps_map_def
+                        Collect_const_mem word_sless_def word_sle_def
+                        ThreadState_Restart_def unat_of_nat mask_def)
+  apply (rule conjI)
+   apply (simp add: Kernel_C.maxIRQ_def word_le_nat_alt ucast_nat_def unat_ucast)
+   apply (cut_tac unat_lt2p[where x="args ! 3"])
+   apply clarsimp
+   apply (clarsimp simp: sysargs_rel_to_n word_less_nat_alt unat_ucast)
+   apply (auto,
+          auto simp: ct_in_state'_def neq_Nil_conv word_bits_def
+                     excaps_in_mem_def slotcap_in_mem_def
+                     cte_wp_at_ctes_of numeral_eqs[symmetric]
+                     valid_tcb_state'_def
+               elim!: pred_tcb'_weakenE
+               dest!: st_tcb_at_idle_thread' interpret_excaps_eq)[1]
+  apply (clarsimp simp: neq_Nil_conv numeral_eqs[symmetric] word_sle_def word_sless_def)
+  apply (drule interpret_excaps_eq[rule_format, where n=0], simp)
+  apply (clarsimp simp: mask_def[where n=4] "StrictC'_thread_state_defs"
+                        rf_sr_ksCurThread ccap_rights_relation_def
+                        rightsFromWord_wordFromRights)
+  apply (simp cong: conj_cong)
+  apply (clarsimp simp: Kernel_C.maxIRQ_def word_le_nat_alt
+                        ucast_nat_def ucast_ucast_mask mask_eq_ucast_eq unat_ucast_mask
+                        less_mask_eq[unfolded word_less_nat_alt])
+  apply (cases "args ! Suc 0 = 0"; clarsimp simp: true_def false_def)
+  done
+
 lemma decodeIRQControlInvocation_ccorres:
-  notes if_cong[cong] tl_drop_1[simp]
+  notes if_cong[cong]
   shows
   "interpret_excaps extraCaps' = excaps_map extraCaps \<Longrightarrow>
    ccorres (intr_and_se_rel \<currency> dc) (liftxf errstate id (K ()) ret__unsigned_long_')
@@ -511,23 +731,23 @@ lemma decodeIRQControlInvocation_ccorres:
                  apply (simp add: split_def invocationCatch_use_injection_handler
                                   injection_handler_bindE bindE_assoc whenE_def
                                   injection_handler_returnOk
-                            del: Collect_const)
+                             del: Collect_const)
                  apply (ctac add: ccorres_injection_handler_csum1
-                    [OF lookupTargetSlot_ccorres, unfolded lookupTargetSlot_def])
+                                  [OF lookupTargetSlot_ccorres, unfolded lookupTargetSlot_def])
                     apply (simp add: Collect_False split_def del: Collect_const)
                     apply csymbr
                     apply (ctac add: ccorres_injection_handler_csum1
-                                       [OF ensureEmptySlot_ccorres])
-                       apply (simp add: injection_handler_returnOk ccorres_invocationCatch_Inr
-                                        performInvocation_def bindE_assoc)
-                       apply (ctac add: setThreadState_ccorres)
-                         apply (ctac(no_vcg) add: invokeIRQControl_ccorres)
-                           apply (rule ccorres_alternative2)
-                           apply (rule ccorres_return_CE, simp+)[1]
-                          apply (rule ccorres_return_C_errorE, simp+)[1]
-                         apply (wp sts_invs_minor')+
-                       apply (simp add: Collect_const_mem)
-                       apply (vcg exspec=setThreadState_modifies)
+                                     [OF ensureEmptySlot_ccorres])
+                      apply (simp add: injection_handler_returnOk ccorres_invocationCatch_Inr
+                                       performInvocation_def bindE_assoc)
+                      apply (ctac add: setThreadState_ccorres)
+                      apply (ctac(no_vcg) add: invokeIRQControl_ccorres)
+                      apply (rule ccorres_alternative2)
+                      apply (rule ccorres_return_CE, simp+)[1]
+                      apply (rule ccorres_return_C_errorE, simp+)[1]
+                      apply (wp sts_invs_minor')+
+                      apply (simp add: Collect_const_mem)
+                      apply (vcg exspec=setThreadState_modifies)
                       apply simp
                       apply (rule ccorres_split_throws)
                        apply (rule ccorres_return_C_errorE, simp+)[1]
@@ -577,7 +797,7 @@ lemma decodeIRQControlInvocation_ccorres:
       apply (rule ccorres_return_CE, simp+)[1]
      apply (rule ccorres_return_C_errorE, simp+)[1]
     apply wp
-   apply vcg
+   apply (vcg exspec=Arch_decodeIRQControlInvocation_modifies)
   apply (simp add: syscall_error_to_H_cases)
   apply (clarsimp simp: interpret_excaps_test_null excaps_map_def
                         Collect_const_mem word_sless_def word_sle_def
