proof/invariant-abstract/ARM/ArchEmptyFail_AI.thy
@@ -23,7 +23,7 @@ crunch_ignore (empty_fail)
         clean_D_PoU_impl cleanInvalidate_D_PoC_impl cleanInvalidateL2Range_impl
         invalidateL2Range_impl cleanL2Range_impl flushBTAC_impl
         writeContextID_impl isb_impl dsb_impl dmb_impl setHardwareASID_impl
-        writeTTBR0_impl cacheRangeOp)
+        writeTTBR0_impl cacheRangeOp setIRQTrigger_impl)
 
 crunch (empty_fail) empty_fail[wp, EmptyFail_AI_assms]:
   loadWord, load_word_offs, storeWord, getRestartPC, get_mrs
