proof/invariant-abstract/ARM_HYP/ArchBCorres2_AI.thy
@@ -54,7 +54,10 @@ lemma transfer_caps_loop_bcorres[wp]:
 
 lemma invoke_irq_control_bcorres[wp]: "bcorres (invoke_irq_control a) (invoke_irq_control a)"
   apply (cases a)
-  apply (wp | simp add: arch_invoke_irq_control_def)+
+  apply wpsimp
+  apply (rename_tac acap)
+  apply (case_tac acap)
+  apply wpsimp
   done
 
 lemma invoke_irq_handler_bcorres[wp]: "bcorres (invoke_irq_handler a) (invoke_irq_handler a)"
