proof/refine/ARM/Arch_R.thy
@@ -1919,7 +1919,7 @@ lemma arch_decodeInvocation_wf[wp]:
                arch_kernel_object.splits)
             apply ((wp whenE_throwError_wp isFinalCapability_inv
                 | wpc |simp add: valid_arch_inv'_def valid_pti'_def if_apply_def2 |
-                  rule hoare_drop_imp)+)[14]
+                  rule hoare_drop_imp)+)[15]
    apply (clarsimp simp: linorder_not_le isCap_simps
                          cte_wp_at_ctes_of diminished_arch_update')
    apply (simp add: valid_cap'_def capAligned_def)
